Schema lemmas for other fupds

theories/base_logic/lib/fupd_level.v
@@ -834,6 +834,12 @@ Definition bi_sch_except_0 (P: bi_schema) : bi_schema :=
 Definition bi_sch_bupd_wand (P1 P2: bi_schema) :=
   bi_sch_wand P1 (bi_sch_bupd P2).
 
+Definition bi_sch_fupd_mj E1 E2 mj (P: bi_schema) : bi_schema :=
+  bi_sch_bupd_wand
+    (bi_sch_sep (bi_sch_wsat) (bi_sch_ownE (λ k, AE k mj ∪ MaybeEn E1)))
+    (bi_sch_except_0 (bi_sch_sep (bi_sch_wsat)
+                                (bi_sch_sep (bi_sch_ownE (λ k, AE k mj ∪ MaybeEn E2)) P))).
+
 Definition bi_sch_fupd E1 E2 (P: bi_schema) : bi_schema :=
   bi_sch_bupd_wand
     (bi_sch_sep (bi_sch_wsat) (bi_sch_ownE (λ k, AE k (Some O) ∪ MaybeEn E1)))
@@ -857,6 +863,25 @@ Lemma bi_sch_fupd_interp E1 E2 lvl Qs Qs_mut Psch P:
   (|lvl,(Some 0)={E1, E2}=> P)%I.
 Proof.
   intros Heq. rewrite uPred_fupd_split_level_eq. by apply bi_sch_fupd_interp'.
+Qed.
+
+Lemma bi_sch_fupd_interp_mj' E1 E2 lvl mj Qs Qs_mut Psch P:
+  bi_schema_interp lvl Qs Qs_mut Psch = P →
+  bi_schema_interp lvl Qs Qs_mut (bi_sch_fupd_mj E1 E2 mj Psch) =
+    (wsat lvl ∗ ownE (AE lvl mj ∪ MaybeEn E1) ==∗ ◇ (wsat lvl ∗ ownE (AE lvl mj ∪ MaybeEn E2) ∗ P))%I.
+Proof.
+  intros Heq.
+  rewrite ?bi_schema_interp_unfold //=.
+  do 11 (rewrite {1}bi_schema_interp_unfold //=).
+  rewrite Heq. rewrite ?bi_schema_interp_unfold //=.
+Qed.
+
+Lemma bi_sch_fupd_interp_mj E1 E2 lvl mj Qs Qs_mut Psch P:
+  bi_schema_interp (S lvl) Qs Qs_mut Psch = P →
+  bi_schema_interp (S lvl) Qs Qs_mut (bi_sch_fupd_mj E1 E2 mj Psch) =
+  (|lvl,mj={E1, E2}=> P)%I.
+Proof.
+  intros Heq. rewrite uPred_fupd_split_level_eq. by apply bi_sch_fupd_interp_mj'.
 Qed.
 
 End schema_test_fupd.
